edge flips only in osteps: a good compromise

coq/open.v
@@ -685,6 +685,16 @@ Proof.
   by case: b.
 Qed.
 
+Lemma add_edge_graph'' (G : pre_graph) e z t v (graph_G : is_graph (G ∔ [e,z,v,t])) x y u :
+  x \in vset G -> y \in vset G -> is_graph (G ∔ [e,x,u,y]).
+Proof.
+  move => xG yG. split => //=; try apply graph_G. 
+  move => e' b; case/fset1UE => [->|[? H]]; rewrite updateE ?(endptP) //.
+  by case: b.
+  generalize (endptP (is_graph:=graph_G) (e:=e') b). 
+  rewrite /=updateE//. move=>D. apply D. by apply fset1Ur. 
+Qed.
+
 Lemma add_edge_graph (G : pre_graph) (graph_G : is_graph G) x y u :
   x \in vset G -> y \in vset G -> is_graph (add_edge G x u y).
 Proof. exact: add_edge_graph'. Qed.
@@ -1081,16 +1091,33 @@ Variant ostep (G : pre_graph) : pre_graph -> Type :=
     oarc G e1 x u y -> oarc G e2 x v y ->
     ostep G ((del_edges G [fset e1;e2]) ∔ [maxn e1 e2,x,u∥v,y]).
 
-Inductive osteps: pre_graph -> pre_graph -> Prop :=
-  | weq_step:    RelationClasses.subrelation weqG osteps
-  | ostep_step:    CRelationClasses.subrelation ostep osteps
-  | osteps_trans : RelationClasses.Transitive osteps.
+(* flipping an edge; this rule is not included in [ostep] as it would make the rewrite system non-terminating 
+   we however use it in [osteps] in order to enable wlog reasonings in the local confluence proof
+   this is fine in the end since fliping edges is allowed in isomorphisms
+
+   it would be even nicer to let weqG handle edge flips ; 
+   it is however convenient to keep weqG in Prop
+   and adding edge flips in Prop prevents us from proving the implication weqG => oiso2 (lemma [weqG_oliso] below, with oiso2 in Type) 
+   this implication is quite convenient in [ostep_of]
+ *)
+Variant fstep: relation pre_graph :=
+| flip_step: forall (G : pre_graph) e x y u v, 
+                      u° ≡ v ->
+                      x \in vset G -> y \in vset G ->
+                      fstep (G ∔ [e,x,u,y])%O (G ∔ [e,y,v,x])%O.
+  
+Inductive osteps: relation pre_graph :=
+| weq_step: RelationClasses.subrelation weqG osteps
+| fstep_step: RelationClasses.subrelation fstep osteps
+| ostep_step: CRelationClasses.subrelation ostep osteps
+| osteps_trans: RelationClasses.Transitive osteps.
 Instance osteps_preorder: PreOrder osteps.
 Proof.
   split. intro. by apply weq_step.
   apply osteps_trans.
 Qed.
 Existing Instance weq_step.
+Existing Instance fstep_step.
 Existing Instance ostep_step.
 
 Lemma weq_stepL G G' H : G ≡G G' -> osteps G' H -> osteps G H.
@@ -1224,25 +1251,36 @@ Proof. by []. Qed.
 
 Ltac e2split := do 2 eexists; split; [split|].
 
-Lemma add_edge_flip (G : pre_graph) (isG : is_graph G) e x y u v: 
-  u° ≡ v ->
-  (* get rid of these assumptions?  *)
-  x \in vset G -> y \in vset G ->
-  G ∔ [e,x,u,y] ≡G G ∔ [e,y,v,x].
-Admitted.
-
 (* Lemma iso2_edge_flip (G : graph2) (x y : G) u : G ∔ [x,u,y] ≃2 G ∔ [y,u°,x]. *)
 (* Proof. apply add_edge2_rev. by apply Eqv'_sym. Defined. *)
 
 (* We prove this directly rather than going though [add_edge2_rev],
 because this way we can avoid the assumption [e \notin eset G] *)
-Lemma add_edge_flip_bak (G : pre_graph) (isG : is_graph G) e x y u v: 
+Lemma add_edge_flip_old (G : pre_graph) (isG : is_graph G) e x y u v: 
   u° ≡ v ->
   x \in vset G -> y \in vset G -> G ∔ [e,x,u,y] ⩭2 G ∔ [e,y,v,x].
 Proof.
   move => E xG yG. 
   have isG1 : is_graph (G ∔ [e,x,u,y]) by apply: add_edge_graph'.
   have isG2 : is_graph (G ∔ [e,y,v,x]) by apply: add_edge_graph'.
+  econstructor.
+  pose dir (e0 : edge (close (G ∔ [e,x,u,y]) isG1)) := val e0 == e.
+  iso2 bij_id bij_id dir => //=. 2-3: exact: val_inj.
+  split => //.
+  - case => e' He' b /=. apply: val_inj => /=. case: (fset1UE He') => [?|].
+    + subst e'. by rewrite /dir/=!eqxx addTb !updateE if_neg. 
+    + case => A ?. by rewrite /dir/= (negbTE A) !updateE.
+  - case => e' He'. rewrite /dir/=. case: (fset1UE He') => [?|].
+    + subst e'. rewrite eqxx !updateE. by symmetry in E.
+    + case => A ?. by rewrite /dir/= (negbTE A) !updateE.
+Defined.
+
+Lemma add_edge_flip (G : pre_graph) e x y u v (isG1 : is_graph (G ∔ [e,x,u,y])): 
+  u° ≡ v ->
+  x \in vset G -> y \in vset G -> G ∔ [e,x,u,y] ⩭2 G ∔ [e,y,v,x].
+Proof.
+  move => E xG yG. 
+  have isG2 : is_graph (G ∔ [e,y,v,x]) by apply: add_edge_graph''.
   econstructor.
   pose dir (e0 : edge (close (G ∔ [e,x,u,y]) isG1)) := val e0 == e.
   iso2 bij_id bij_id dir => //=. 2-3: exact: val_inj.
@@ -1535,7 +1573,7 @@ Proof with eauto with typeclass_instances.
         rewrite -> oarc_cnv in arc_e1',arc_e2'. 
         move/(_ y' x' yDz' xDz' _ _ _ _ arc_e2' arc_e1') in W. rewrite fsetUC eq_sym in W.
         case: W => // Gl [Gr] [[S1 S2] WG]. exists Gl. exists Gr. do 2 (split => //).
-        rewrite maxnC add_edge_flip; eauto with vset. 
+        rewrite-> maxnC, flip_step; eauto with vset. 
         by rewrite !cnvdot cnvtst dotA. }
       subst y'. 
       have ? : e2' = e by apply: oarc_uniqeR arc_e2'. subst e2'. 
@@ -1639,7 +1677,7 @@ Proof with eauto with typeclass_instances.
           case: W => //. 1-2: by rewrite <- oarc_cnv. 
           move => Gl [Gr] [[S1 S2] E']. e2split;[exact: S1| |exact: E']. 
           (* TODO: this is exactly the same as in the first wlog argument -> lemma *)
-          rewrite maxnC add_edge_flip; eauto with vset.
+          rewrite-> maxnC, flip_step; eauto with vset.
           by rewrite !cnvdot cnvtst dotA. }
         subst e1' e2'.
         case: (altP (z =P z')) => [?|D].
@@ -1714,7 +1752,7 @@ Proof with eauto with typeclass_instances.
          rewrite -> oarc_cnv in arc_e1,arc_e2. 
          move/(_ _ _ _ _ _ _ arc_e2 arc_e1) in W. rewrite fsetUC eq_sym in W.
          case: W => // Gl [Gr] [[S1 S2] WG]. exists Gl. exists Gr. do 2 (split => //). 
-         rewrite maxnC add_edge_flip; eauto with vset.
+         rewrite-> maxnC, flip_step; eauto with vset.
          by rewrite !cnvdot cnvtst dotA. }
        wlog ? : e1' e2' x' y' u' v'  arc_e1' arc_e2' Iz' e1De2' xDz' yDz' He / e2 = e1' ; [move => W|subst e1'].
        { have: e2 \in [fset e1';e2']. { move/fsetP : He => /(_ e2). rewrite in_fset1 eqxx. by case/fsetIP. }
@@ -1722,7 +1760,7 @@ Proof with eauto with typeclass_instances.
          rewrite -> oarc_cnv in arc_e1',arc_e2'. 
          move/(_ _ _ _ _ _ _ arc_e2' arc_e1') in W. rewrite fsetUC eq_sym in W.
          case: W => // Gl [Gr] [[S1 S2] WG]. exists Gl. exists Gr. do 2 (split => //). 
-         rewrite maxnC add_edge_flip; eauto with vset.
+         rewrite-> maxnC, flip_step; eauto with vset.
          by rewrite !cnvdot cnvtst dotA. }
        have {He} E1 : e1 != e2'.
        { apply: contraNneq e1De2 => E. by rewrite -in_fset1 -He !inE E !eqxx. }
@@ -1778,7 +1816,7 @@ Proof with eauto with typeclass_instances.
         subst x'. rewrite -> oarc_cnv in arc_e2', arc_e1'. 
         case: (W _ _ _ _ _ _ _ arc_e2' arc_e1'); rewrite 1?eq_sym //.
         move => Gl' [Gr'] [[Sl Sr] E]. e2split; [exact: Sl| |exact: E].
-        rewrite fsetUC maxnC add_edge_flip; eauto with vset.
+        rewrite-> fsetUC, maxnC, flip_step; eauto with vset.
         by rewrite cnvpar parC. }
       subst y'. 
       wlog ? : e1 e2 u v x y e1De2 arc_e1 arc_e2 xDz yDz Iz / e1' = e1.
@@ -1787,7 +1825,7 @@ Proof with eauto with typeclass_instances.
         subst e1'. rewrite -> oarc_cnv in arc_e2, arc_e1. 
         case: (W _ _ _ _ _ _ _ arc_e2 arc_e1); rewrite // 1?eq_sym 1?fsetUC //.
         move => Gl [Gr] [[Sl Sr] E]. e2split; [ | exact: Sr|exact: E].
-        rewrite maxnC add_edge_flip; eauto with vset.
+        rewrite->maxnC, flip_step; eauto with vset.
         by rewrite !cnvdot cnvtst dotA. }
       subst e1'. 
       have /eqP ? : e2' == e2; [|subst e2'].
@@ -1897,7 +1935,7 @@ Proof with eauto with typeclass_instances.
         subst x' y'. rewrite -> oarc_cnv in arc_e2'. case: (W _ _ u'° _ arc_e2') => //.
         move => Gl [Gr] [[Sl Sr] EG]. 
         e2split; [exact: Sl| |exact: EG]. 
-        rewrite add_edge_flip; eauto with vset. by rewrite cnvpar. }
+        rewrite-> flip_step; eauto with vset. by rewrite cnvpar. }
       subst x' y'. 
       (* There are actually two cases here *)
       have [Hv|[? Hv]]: ((v ≡ v') \/ (x = y /\ v ≡ v'°)).
@@ -1940,7 +1978,7 @@ Proof with eauto with typeclass_instances.
         rewrite -> oarc_cnv in arc_e1,arc_e2. 
         move/(_ _ _ _ _ _ _ arc_e2 arc_e1) in W. rewrite fsetUC eq_sym in W.
         case: W => // Gl [Gr] [[S1 S2] WG]. exists Gl. exists Gr. do 2 (split => //). 
-        rewrite maxnC add_edge_flip; eauto with vset.
+        rewrite-> maxnC, flip_step; eauto with vset.
         by rewrite !cnvpar parC. }
       wlog ? : e1' e2' x' y' u' v'  arc_e1' arc_e2' e1De2' He / e2 = e1' ; [move => W|subst e1'].
       { have: e2 \in [fset e1';e2']. { move/fsetP : He => /(_ e2). rewrite in_fset1 eqxx. by case/fsetIP. }
@@ -1948,7 +1986,7 @@ Proof with eauto with typeclass_instances.
         rewrite -> oarc_cnv in arc_e1',arc_e2'. 
         move/(_ _ _ _ _ _ _ arc_e2' arc_e1') in W. rewrite eq_sym [[fset e2';_]]fsetUC in W.
         case: W => // Gl [Gr] [[S1 S2] WG]. exists Gl. exists Gr. do 2 (split => //).
-        rewrite maxnC add_edge_flip; eauto with vset.
+        rewrite-> maxnC, flip_step; eauto with vset.
         by rewrite !cnvpar parC. }
       have {He} E1 : e1 != e2'.
       { apply: contraNneq e1De2 => E. by rewrite -in_fset1 -He !inE E !eqxx. }
@@ -1958,7 +1996,7 @@ Proof with eauto with typeclass_instances.
         rewrite -> oarc_cnv in arc_e2'. subst x' y'.  
         case: (W _ _ u'° _ arc_e2'). split => //. by rewrite E cnvI.
         move => Gl [Gr] [[Sl Sr] EG]. e2split; [exact: Sl| |exact: EG].
-        rewrite add_edge_flip; eauto with vset.
+        rewrite->flip_step; eauto with vset.
         by rewrite !cnvpar. }
       subst.
       have He2' : e2' \notin [fset e1; e2] by rewrite !inE negb_or ![e2' == _]eq_sym E1 e1De2'.
@@ -2003,6 +2041,7 @@ Lemma osteps_graph (F G : pre_graph) (isG : is_graph F) : osteps F G -> is_graph
 Proof.
   move => S. elim: S isG => {F G}. 
   - move => F G FG H. by eauto using weqG_graph.
+  - move => F G FG H. destruct FG. eauto using add_edge_graph''. 
   - move => F G FG isF. apply: ostep_graph FG.
   - move => F G H. tauto.
 Qed.
@@ -2384,8 +2423,10 @@ Qed.
 
 Lemma osteps_iso (F G H: pre_graph): osteps F H -> F ⩭2 G -> exists U, osteps G U /\ inhabited (H ⩭2 U).
 Proof.
-  intro S. revert G. induction S as [F G FG|F G FG|F G H FG IH GH IH']; intros F' FF'.
+  intro S. revert G. induction S as [F G FG|F G FG|F G FG|F G H FG IH GH IH']; intros F' FF'.
   - exists F'. split. by []. exists. transitivity F=>//. symmetry. apply weqG_iso2L=>//. apply FF'.
+  - exists F'. split=>//. destruct FG. exists. etransitivity. 2: eassumption.
+    symmetry. apply add_edge_flip=>//. apply FF'. 
   - destruct (ostep_iso FG FF') as [U [F'U GU]]. exists U. split. by apply ostep_step. by exists.
   - destruct (IH _ FF') as [G' [F'G' [GG']]]. 
     destruct (IH' _ GG') as [H' [G'H' [HH']]]. 
@@ -2910,10 +2951,11 @@ Qed.
 Lemma steps_of (G H : pre_graph) (isG : is_graph G) (isH : is_graph H) : 
   osteps G H -> steps (close G) (close H).
 Proof.
-  move => S. elim: S isG isH => {G H} [G H h|G H GH |G F H S IH1 _ IH2] isG isH.
+  move => S. elim: S isG isH => {G H} [G H h|G H GH|G H GH|G F H S IH1 _ IH2] isG isH.
   - apply: iso_step.
     apply (weqG_iso2L isG) in h.
     apply: iso2_comp (iso2_comp (oiso2_iso h) _); apply: close_irrelevance.
+  - destruct GH. apply iso_step. apply liso_of_oliso. apply add_edge_flip=>//.
   - exact: steps_of_ostep.
   - have isF : is_graph F by apply: osteps_graph S. 
     by transitivity (close F). 
